Weidenbach_Book/IsaSAT.thy
@@ -28,17 +28,35 @@ definition SAT :: \<open>nat clauses \<Rightarrow> nat cdcl\<^sub>W_restart_mset
 definition (in -) SAT_wl :: \<open>nat clause_l list \<Rightarrow> nat twl_st_wl nres\<close> where
   \<open>SAT_wl CS = do{
     let \<A>\<^sub>i\<^sub>n' = extract_atms_clss CS {};
-    let S = isasat_input_ops.init_state_wl (mset_set \<A>\<^sub>i\<^sub>n');
-    T \<leftarrow> init_dt_wl CS (to_init_state S);
-    let T = from_init_state T;
-    if get_conflict_wl T \<noteq> None
-    then RETURN T
-    else if CS = [] then RETURN (([], fmempty, None, {#}, {#}, {#}, \<lambda>_. undefined))
-    else do {
-       ASSERT (extract_atms_clss CS {} \<noteq> {});
-       ASSERT(isasat_input_bounded_nempty (mset_set \<A>\<^sub>i\<^sub>n'));
-       isasat_input_ops.cdcl_twl_stgy_prog_wl_D (mset_set \<A>\<^sub>i\<^sub>n') (finalise_init T)
-    }
+    b \<leftarrow> SPEC(\<lambda>_. True);
+    if b then do {
+      let S = isasat_input_ops.init_state_wl (mset_set \<A>\<^sub>i\<^sub>n');
+      T \<leftarrow> init_dt_wl CS (to_init_state S);
+      let T = from_init_state T;
+      if get_conflict_wl T \<noteq> None
+      then RETURN T
+      else if CS = [] then RETURN (([], fmempty, None, {#}, {#}, {#}, \<lambda>_. undefined))
+      else do {
+         ASSERT (extract_atms_clss CS {} \<noteq> {});
+         ASSERT(isasat_input_bounded_nempty (mset_set \<A>\<^sub>i\<^sub>n'));
+         ASSERT(mset `# ran_mf (get_clauses_wl T) + get_unit_clauses_wl T = mset `# mset CS);
+         isasat_input_ops.cdcl_twl_stgy_prog_break_wl_D (mset_set \<A>\<^sub>i\<^sub>n') P (finalise_init T)
+      }
+   }
+   else do {
+      let S = isasat_input_ops.init_state_wl (mset_set \<A>\<^sub>i\<^sub>n');
+      T \<leftarrow> init_dt_wl CS (to_init_state S);
+      let T = from_init_state T;
+      if get_conflict_wl T \<noteq> None
+      then RETURN T
+      else if CS = [] then RETURN (([], fmempty, None, {#}, {#}, {#}, \<lambda>_. undefined))
+      else do {
+         ASSERT (extract_atms_clss CS {} \<noteq> {});
+         ASSERT(isasat_input_bounded_nempty (mset_set \<A>\<^sub>i\<^sub>n'));
+         ASSERT(mset `# ran_mf (get_clauses_wl T) + get_unit_clauses_wl T = mset `# mset CS);
+         isasat_input_ops.cdcl_twl_stgy_prog_wl_D (mset_set \<A>\<^sub>i\<^sub>n') (finalise_init T)
+      }
+   }
   }\<close>
 
 
@@ -72,6 +90,7 @@ definition IsaSAT :: \<open>nat clause_l list \<Rightarrow> nat literal list opt
       else do {
          ASSERT(\<A>\<^sub>i\<^sub>n' \<noteq> {#});
          ASSERT(isasat_input_bounded_nempty \<A>\<^sub>i\<^sub>n');
+         ASSERT(mset `# ran_mf (get_clauses_wl T) + get_unit_clauses_wl T = mset `# mset CS);
          let T = finalise_init T;
          U \<leftarrow> isasat_input_ops.cdcl_twl_stgy_prog_break_wl_D \<A>\<^sub>i\<^sub>n' isasat_fast_wl T;
          RETURN (if get_conflict_wl U = None then extract_model_of_state U else extract_stats U)
@@ -88,6 +107,7 @@ definition IsaSAT :: \<open>nat clause_l list \<Rightarrow> nat literal list opt
       else do {
          ASSERT(\<A>\<^sub>i\<^sub>n' \<noteq> {#});
          ASSERT(isasat_input_bounded_nempty \<A>\<^sub>i\<^sub>n');
+         ASSERT(mset `# ran_mf (get_clauses_wl T) + get_unit_clauses_wl T = mset `# mset CS);
          let T = finalise_init T;
          U \<leftarrow> isasat_input_ops.cdcl_twl_stgy_prog_wl_D \<A>\<^sub>i\<^sub>n' T;
          RETURN (if get_conflict_wl U = None then extract_model_of_state U else extract_stats U)
@@ -131,6 +151,11 @@ lemma empty_init_code_hnr[sepref_fr_rules]:
   by sepref_to_hoare (sep_auto simp: empty_conflict_code_def empty_conflict_def
        hr_comp_def empty_init_code_def)
 
+text \<open>
+  This is a trick to recover from consumption of a variable (\<^term>\<open>\<A>\<^sub>i\<^sub>n\<close>) that is passed as
+  argument and destroyed by the initialisation: We copy it as a zero-cost 
+  (by creating a \<^term>\<open>()\<close>), because we don't need it in the code and only in the specification.
+\<close>
 definition virtual_copy where
   [simp]: \<open>virtual_copy = id\<close>
 
@@ -225,6 +250,7 @@ definition IsaSAT_heur :: \<open>nat clause_l list \<Rightarrow> (nat literal li
         else do {
            ASSERT(\<A>\<^sub>i\<^sub>n'' \<noteq> {#});
            ASSERT(isasat_input_bounded_nempty \<A>\<^sub>i\<^sub>n'');
+           ASSERT(mset `# ran_mf (get_clauses_wl_heur_init T) \<subseteq># mset `# mset CS);
            ASSERT((\<lambda>(M', N', D', Q', W', ((ns, m, fst_As, lst_As, next_search), to_remove), \<phi>, clvls). fst_As \<noteq> None \<and>
              lst_As \<noteq> None) T);
            T \<leftarrow> finalise_init_code (T::twl_st_wl_heur_init);
@@ -244,6 +270,7 @@ definition IsaSAT_heur :: \<open>nat clause_l list \<Rightarrow> (nat literal li
         else do {
            ASSERT(\<A>\<^sub>i\<^sub>n'' \<noteq> {#});
            ASSERT(isasat_input_bounded_nempty \<A>\<^sub>i\<^sub>n'');
+           ASSERT(mset `# ran_mf (get_clauses_wl_heur_init T) \<subseteq># mset `# mset CS);
            ASSERT((\<lambda>(M', N', D', Q', W', ((ns, m, fst_As, lst_As, next_search), to_remove), \<phi>, clvls). fst_As \<noteq> None \<and>
              lst_As \<noteq> None) T);
            T \<leftarrow> finalise_init_code (T::twl_st_wl_heur_init);
@@ -435,9 +462,8 @@ sepref_register to_init_state from_init_state get_conflict_wl_is_None_init extra
   isasat_input_ops.init_dt_wl_heur
 declare init_state_wl_heur_hnr[to_hnr, OF refl, sepref_fr_rules]
   init_dt_wl_code.refine[sepref_fr_rules]
- isasat_input_ops.get_stats_code[sepref_fr_rules]
- init_state_wl_heur_fast_hnr[to_hnr, OF refl, sepref_fr_rules]
-thm init_state_wl_heur_hnr[to_hnr, OF refl, sepref_fr_rules]
+  isasat_input_ops.get_stats_code[sepref_fr_rules]
+  init_state_wl_heur_fast_hnr[to_hnr, OF refl, sepref_fr_rules]
 
 lemma uint_max_nat_assn_hnr[sepref_fr_rules]:
   \<open>(uncurry0 (return uint_max), uncurry0 (RETURN uint_max)) \<in> unit_assn\<^sup>k \<rightarrow>\<^sub>a nat_assn\<close>
@@ -465,7 +491,7 @@ sepref_definition IsaSAT_code
   isasat_input_bounded.get_conflict_wl_is_None_init_wl_hnr[
     unfolded get_conflict_wl_is_None_init_def[symmetric], sepref_fr_rules]
   supply id_mset_list_assn_list_mset_assn[sepref_fr_rules] get_conflict_wl_is_None_def[simp]
-   option.splits[split] virtual_copy_def[simp]
+   option.splits[split]
    extract_stats_def[simp del]
   apply (rewrite at \<open>extract_atms_clss _ \<hole>\<close> op_extract_list_empty_def[symmetric])
   by sepref
@@ -475,19 +501,16 @@ definition nth_u_code' where
 
 code_printing constant nth_u_code' \<rightharpoonup> (SML) "(fn/ ()/ =>/ Array.sub/ ((_),/ Word32.toInt (_)))"
 
-
 definition nth_u64_code' where
   [symmetric, code]: \<open>nth_u64_code' = nth_u64_code\<close>
 
 code_printing constant nth_u64_code' \<rightharpoonup> (SML) "(fn/ ()/ =>/ Array.sub/ ((_),/ Uint64.toFixedInt (_)))"
-
 
 definition heap_array_set'_u' where
   [symmetric, code]: \<open>heap_array_set'_u' = heap_array_set'_u\<close>
 
 code_printing constant heap_array_set'_u' \<rightharpoonup>
    (SML) "(fn/ ()/ =>/ Array.update/ ((_),/ (Word32.toInt (_)),/ (_)))"
-
 
 definition heap_array_set'_u64' where
   [symmetric, code]: \<open>heap_array_set'_u64' = heap_array_set'_u64\<close>
@@ -507,9 +530,6 @@ definition length_aa_u_code' where
 
 code_printing constant length_aa_u_code' \<rightharpoonup> (SML_imp)
    "(fn/ ()/ =>/ Word32.fromInt (Array.length (Array.sub/ ((fn/ (a,b)/ =>/ a) (_),/ IntInf.toInt (integer'_of'_nat (_))))))"
-
-term delete_index_and_swap_code
-term nth_raa_i_u64
 
 definition nth_raa_i_u64' where
   [symmetric, code]: \<open>nth_raa_i_u64' = nth_raa_i_u64\<close>
@@ -812,7 +832,10 @@ proof -
                      CS \<noteq> {#} \<and>
                      conflicting U \<noteq> None \<and>
                      backtrack_lvl U = 0 \<and> unsatisfiable (set_mset CS)))\<close>
-   (is \<open>_ \<le> \<Down> _ ?Spec\<close>)
+      (is ?steps is \<open>_ \<le> \<Down> _ ?Spec\<close>) and
+    clauses: \<open>mset `# ran_mf (get_clauses_wl (fst T)) +
+         get_unit_clauses_wl (fst T) = mset `# mset CS'\<close>
+        (is ?clss)
     if
       CS_p: \<open>Multiset.Ball CS distinct_mset \<and> (\<forall>C\<in>#CS. \<forall>L\<in>#C. nat_of_lit L \<le> uint_max)\<close> and
       CS'_CS: \<open>(CS', CS) \<in> list_mset_rel O \<langle>list_mset_rel\<rangle>mset_rel\<close> and
@@ -843,8 +866,7 @@ proof -
       stgy_invs: \<open>twl_stgy_invs (fst W)\<close> and
       snd_T_conflict: \<open>other_clauses_l_init V \<noteq> {#} \<longrightarrow> get_conflict_l_init V \<noteq> None\<close> and
       false_in_conflict: \<open>{#} \<in># mset `# mset CS' \<longrightarrow> get_conflict_l_init V \<noteq> None\<close> and
-      \<open>get_conflict_l_init U \<noteq> None \<longrightarrow>
-       get_conflict_l_init U = get_conflict_l_init V\<close>
+      \<open>get_conflict_l_init U \<noteq> None \<longrightarrow> get_conflict_l_init U = get_conflict_l_init V\<close>
       using spec unfolding init_dt_wl_spec_def init_dt_spec_def apply -
       apply normalize_goal+
       by presburger
@@ -944,7 +966,6 @@ proof -
         by (auto simp: K)
       then have 2: \<open>cdcl\<^sub>W_restart_mset.cdcl\<^sub>W_stgy ?int ?final\<close>
         by (auto simp add: K C_def dest!: cdcl\<^sub>W_restart_mset.cdcl\<^sub>W_stgy.propagate')
-
 
       show ?case
         apply (rule rtranclp.rtrancl_into_rtrancl[OF 1])
@@ -1069,7 +1090,7 @@ proof -
           by (auto simp: CS twl_st_init twl_st)
       qed
     qed
-    show ?thesis
+    show ?steps
       unfolding TWL_to_clauses_state_conv_def from_init_state_def[symmetric]
       apply (rule order_trans)
        apply (rule 2)
@@ -1079,7 +1100,11 @@ proof -
        apply (rule conclusive_le)
       apply simp
       done
-    qed
+    show ?clss
+      using clss U unfolding all_clss_lf_ran_m
+      by (cases U)
+        (auto simp: S\<^sub>0 state_wl_l_init_def state_wl_l_def N_NE)
+  qed
 
   have init: \<open>init_dt_wl_pre CS' (([], fmempty, None, {#}, {#}, {#}, \<lambda>_. []), {#})\<close>
     if \<open>Ball (set CS') distinct\<close> for CS'
@@ -1109,6 +1134,7 @@ proof -
       subgoal by (rule extract_atms_clss_not_nil)
       subgoal by (auto simp: in_list_mset_rel in_list_mset_rel_mset_rel K
          isasat_input_bounded_nempty_def isasat_input_bounded_nempty_axioms_def)
+      subgoal by (rule clauses)
       subgoal by (rule CDCL_steps)
       subgoal by (rule init) (auto simp: in_list_mset_rel in_list_mset_rel_mset_rel)
       done
@@ -1207,6 +1233,48 @@ lemma (in isasat_input_ops) twl_st_heur_init_wl:
   by (cases T; cases Ta)
     (auto simp: twl_st_heur_init_def twl_st_heur_init_wl_def from_init_state_def)
 
+lemma(in isasat_input_ops) get_clauses_wl_from_init_get_clauses_wl_heur_init:
+  \<open>(T, Ta) \<in> twl_st_heur_init \<Longrightarrow> get_clauses_wl (from_init_state Ta) = get_clauses_wl_heur_init T\<close>
+  by (cases T; cases Ta)
+    (auto simp: twl_st_heur_init_def twl_st_heur_init_wl_def from_init_state_def)
+
+(* TODO Move *)
+lemma (in -) packed_Max_dom_size:
+  assumes p: \<open>packed N\<close>
+  shows \<open>Max_dom N = size (dom_m N)\<close>
+proof -
+  have 1: \<open>dom_m N = mset [1..<Suc (Max_dom N)]\<close>
+    using p unfolding packed_def Max_dom_def[symmetric] .
+  have \<open>size (dom_m N) = size (mset [1..<Suc (Max_dom N)])\<close>
+    unfolding 1 ..
+  also have \<open>\<dots> = length [1..<Suc (Max_dom N)]\<close>
+    unfolding size_mset ..
+  also have \<open>\<dots> = Max_dom N\<close>
+    unfolding length_upt by simp
+  finally show ?thesis
+    by simp
+qed
+
+lemma (in -) Max_dom_le:
+  \<open>L \<in># dom_m N \<Longrightarrow> L \<le> Max_dom N\<close>
+  by (auto simp: Max_dom_def)
+
+lemma isasat_input_bounded_nempty_cdcl_twl_stgy_prog_wl_D_heur_break_cdcl_twl_stgy_prog_wl_D':
+  \<open>isasat_input_bounded_nempty \<A> \<Longrightarrow>
+(S, S') \<in> isasat_input_ops.twl_st_heur \<A> \<Longrightarrow> \<A> = \<A>' \<Longrightarrow>
+isasat_input_ops.cdcl_twl_stgy_prog_break_wl_D_heur_break \<A> S
+\<le> \<Down> (isasat_input_ops.twl_st_heur \<A>)
+    (isasat_input_ops.cdcl_twl_stgy_prog_break_wl_D \<A>' isasat_fast_wl S')\<close>
+  using  isasat_input_bounded_nempty.cdcl_twl_stgy_prog_wl_D_heur_break_cdcl_twl_stgy_prog_wl_D
+             [THEN fref_to_Down, unfolded comp_def, of \<A> S S']
+  by fast
+
+lemma (in isasat_input_ops) get_conflict_wl_is_None_heur_init_get_conflict_wl_is_None_init:
+  \<open>(T, Ta) \<in> twl_st_heur_init  \<Longrightarrow>
+    get_conflict_wl_is_None_heur_init T \<longleftrightarrow> get_conflict_wl_is_None_init (from_init_state Ta)\<close>
+  by (auto simp: )
+(* End Move *)
+
 lemma IsaSAT_heur_IsaSAT: \<open>(IsaSAT_heur, IsaSAT) \<in>
      [\<lambda>CS.  Multiset.Ball (mset CS) distinct \<and> (\<forall>C\<in>set CS. \<forall>L\<in>set C. nat_of_lit L \<le> uint_max)]\<^sub>f
      Id \<rightarrow> \<langle>{((M, stat), M'). M = M'}\<rangle>nres_rel\<close>
@@ -1229,6 +1297,7 @@ proof -
         else do {
            ASSERT(\<A>\<^sub>i\<^sub>n'' \<noteq> {#});
            ASSERT(isasat_input_bounded_nempty \<A>\<^sub>i\<^sub>n'');
+           ASSERT(mset `# ran_mf (get_clauses_wl_heur_init T) \<subseteq># mset `# mset CS);
            ASSERT((\<lambda>(M', N', D', Q', W', ((ns, m, fst_As, lst_As, next_search), to_remove), \<phi>, clvls). fst_As \<noteq> None \<and>
              lst_As \<noteq> None) T);
            T \<leftarrow> finalise_init_code (T::twl_st_wl_heur_init);
@@ -1248,6 +1317,7 @@ proof -
         else do {
            ASSERT(\<A>\<^sub>i\<^sub>n'' \<noteq> {#});
            ASSERT(isasat_input_bounded_nempty \<A>\<^sub>i\<^sub>n'');
+           ASSERT(mset `# ran_mf (get_clauses_wl_heur_init T) \<subseteq># mset `# mset CS);
            ASSERT((\<lambda>(M', N', D', Q', W', ((ns, m, fst_As, lst_As, next_search), to_remove), \<phi>, clvls). fst_As \<noteq> None \<and>
              lst_As \<noteq> None) T);
            T \<leftarrow> finalise_init_code (T::twl_st_wl_heur_init);
@@ -1289,8 +1359,7 @@ proof -
     (is \<open>_ \<Longrightarrow> _ \<le> \<Down> ?init _\<close>)
     for T T' N
     by (auto simp: f_def to_init_state_def)
-  have init: \<open>isasat_input_ops.init_dt_wl_heur (mset_set (extract_atms_clss CS {})) CS
-       T'
+  have init: \<open>isasat_input_ops.init_dt_wl_heur (mset_set (extract_atms_clss CS {})) CS T'
       \<le> \<Down> (isasat_input_ops.twl_st_heur_init (mset_set (extract_atms_clss CS' {})))
           (init_dt_wl CS'
              (to_init_state (isasat_input_ops.init_state_wl (mset_set (extract_atms_clss CS' {})))))\<close>
@@ -1300,10 +1369,8 @@ proof -
       bounded: \<open>isasat_input_bounded (mset_set (extract_atms_clss CS' {}))\<close> and
       TT': \<open>inres (f T) T'\<close> and
       T': \<open>(T', to_init_state (isasat_input_ops.init_state_wl (mset_set (extract_atms_clss CS' {}))))
-     \<in> {(T, T', OS).
-         (T, T')
-         \<in> isasat_input_ops.twl_st_heur_init_wl
-             (mset_set (extract_atms_clss CS' {}))}\<close>
+        \<in> {(T, T', OS). 
+          (T, T') \<in> isasat_input_ops.twl_st_heur_init_wl (mset_set (extract_atms_clss CS' {}))}\<close>
     for CS CS' T T'
   proof -
     have SS': \<open>CS = CS'\<close>
@@ -1334,9 +1401,7 @@ proof -
   have from_init_state: \<open>f T \<le> \<Down> (isasat_input_ops.twl_st_heur_init_wl (mset_set (extract_atms_clss CS' {})))
           (RETURN (from_init_state T'))\<close>
     if
-      TT': \<open>(T, T')
-     \<in> isasat_input_ops.twl_st_heur_init
-         (mset_set (extract_atms_clss CS' {}))\<close>
+      TT': \<open>(T, T') \<in> isasat_input_ops.twl_st_heur_init (mset_set (extract_atms_clss CS' {}))\<close>
     for T T' CS CS'
   proof -
     show ?thesis
@@ -1344,6 +1409,60 @@ proof -
       unfolding f_def
       by (auto simp: isasat_input_ops.twl_st_heur_init_def from_init_state_def
          isasat_input_ops.twl_st_heur_init_wl_def)
+  qed
+  have dom_m_le_uint_max: \<open>\<forall>L\<in>#dom_m (get_clauses_wl_heur U). L < uint_max\<close>
+    if 
+      CS_CS': \<open>(CS, CS') \<in> Id\<close> and
+      length_CS': \<open>b \<and> length CS' < uint_max - 1\<close> and
+      S_fS': \<open>inres (f S') S\<close> and
+      SS': \<open>(S, to_init_state
+            (isasat_input_ops.init_state_wl
+              (mset_set (extract_atms_clss CS' {}))))
+      \<in> {(T, T', OS). (T, T') \<in> isasat_input_ops.twl_st_heur_init_wl
+            (mset_set (extract_atms_clss CS' {}))}\<close> and
+      TU': \<open>(T, U') \<in> isasat_input_ops.twl_st_heur_init
+          (mset_set (extract_atms_clss CS' {}))\<close> and
+      not_none: \<open>case T of
+      (M', N', D', Q', W', xa, xb) \<Rightarrow>
+        (case xa of
+          (x, xa) \<Rightarrow>
+            (case x of
+            (ns, m, fst_As, lst_As, next_search) \<Rightarrow>
+              \<lambda>to_remove (\<phi>, clvls). fst_As \<noteq> None \<and> lst_As \<noteq> None)
+            xa)
+          xb\<close> and
+      UT: \<open>inres (finalise_init_code T) U\<close> and
+      UU': \<open>(U, finalise_init (from_init_state U'))
+      \<in> isasat_input_ops.twl_st_heur (mset_set (extract_atms_clss CS' {}))\<close> and
+      dom: \<open>mset `# ran_mf (get_clauses_wl_heur_init T) \<subseteq># mset `# mset CS\<close>
+    for CS CS' b S' S T U' U
+  proof -
+    obtain M N D R where
+      \<open>S = (M, N, D, R)\<close>
+      by (cases S) auto
+    have \<open>size (dom_m N) \<le> size (mset `# ran_mf N)\<close> for N
+      by (auto simp: dom_m_def ran_m_def)
+    moreover have 1: \<open>packed N \<Longrightarrow> Max_dom N = size (dom_m N)\<close> for N
+      by (rule packed_Max_dom_size)
+    moreover {
+      have \<open>size (dom_m (get_clauses_wl_heur_init T)) \<le> size (ran_mf (get_clauses_wl_heur_init T))\<close>
+        by (auto simp: ran_m_def)
+      moreover have \<open>size (ran_mf (get_clauses_wl_heur_init T)) \<le> length CS\<close> 
+        using size_mset_mono[OF dom] by auto 
+      ultimately have \<open>size (dom_m (get_clauses_wl_heur_init T)) \<le> uint_max - 1\<close>
+        using length_CS' CS_CS' by force
+    }
+    ultimately have H: \<open>L < uint_max\<close>
+      if packed: \<open>packed (get_clauses_wl_heur_init T)\<close> and \<open>L \<in># dom_m (get_clauses_wl_heur_init T)\<close> for L
+      using length_CS' that Max_dom_le[of L \<open>get_clauses_wl_heur_init T\<close>]
+       1[OF packed] dom
+      by auto
+    show ?thesis
+      using UU' UT TU' not_none dom H
+      by (cases U; cases U'; cases T)
+        (auto simp: finalise_init_code_def take1_def from_init_state_def finalise_init_def
+        inres_def isasat_input_ops.twl_st_heur_def isasat_input_ops.twl_st_heur_init_wl_def
+        isasat_input_ops.twl_st_heur_init_def)
   qed
   show ?thesis
     supply RETURN_as_SPEC_refine[refine2 del]
@@ -1356,8 +1475,7 @@ proof -
            isasat_input_ops.finalise_init_finalise_init[THEN fref_to_Down, unfolded comp_def]
            isasat_input_bounded_nempty.cdcl_twl_stgy_prog_wl_D_heur_cdcl_twl_stgy_prog_wl_D
              [THEN fref_to_Down_explode, unfolded comp_def]
-           isasat_input_bounded_nempty.cdcl_twl_stgy_prog_wl_D_heur_break_cdcl_twl_stgy_prog_wl_D
-             [THEN fref_to_Down, unfolded comp_def])
+           isasat_input_bounded_nempty_cdcl_twl_stgy_prog_wl_D_heur_break_cdcl_twl_stgy_prog_wl_D')
     subgoal by auto
     subgoal by auto
     subgoal by auto
@@ -1375,6 +1493,10 @@ proof -
       by (auto simp: empty_conflict_code_def)
     subgoal by auto
     subgoal by auto
+    subgoal (*TODO tune proof*)
+      apply (auto simp: isasat_input_ops.get_clauses_wl_from_init_get_clauses_wl_heur_init
+        intro: mset_subset_eq_add_left)
+      by (metis mset_subset_eq_add_left)
     subgoal
       by (auto dest: isasat_input_ops.twl_st_heur_init_vmtf_next_emptyD)
     subgoal
@@ -1385,40 +1507,51 @@ proof -
     apply assumption+
     subgoal
       by (rule isasat_input_ops.twl_st_heur_init_wl)
-    subgoal
-      sorry
-    supply [[unify_trace_failure]]
-    apply (rule isasat_input_bounded_nempty.cdcl_twl_stgy_prog_wl_D_heur_break_cdcl_twl_stgy_prog_wl_D
-             [THEN fref_to_Down, unfolded comp_def])
-    thm isasat_input_bounded_nempty.cdcl_twl_stgy_prog_wl_D_heur_break_cdcl_twl_stgy_prog_wl_D
-             [THEN fref_to_Down, unfolded comp_def]
-oops
+    subgoal for CS CS' b S' S T U' U
+      by (rule dom_m_le_uint_max)
+    subgoal by fast
+    subgoal by fast
     subgoal premises p
-      using p(26) \<comment> \<open>only last assumption\<close>
+      using p(30)
       by (auto simp: extract_model_of_state_stat_def extract_model_of_state_def
           isasat_input_ops.twl_st_heur_def get_conflict_wl_is_None_heur_def
           get_conflict_wl_is_None_heur_init_def extract_state_stat_def
           get_conflict_wl_is_None_def split: option.splits)
-    subgoal
-      by (auto simp:  isasat_input_ops.twl_st_heur_init_wl_def
-          get_conflict_wl_is_None_heur_init_def get_conflict_wl_is_None_init_def
-          get_conflict_wl_is_None_def split: option.splits)
-    oops
+    subgoal by auto
     apply assumption+
-    subgoal ..
+    subgoal by fast
+    apply assumption+
     subgoal by simp
+    subgoal premises p by (simp add: empty_init_code_def)
     subgoal by simp
+    subgoal premises p by (simp add: empty_conflict_code_def)
+    subgoal by auto
+    subgoal by auto
+    subgoal (*TODO tune proof*)
+      apply (auto simp: isasat_input_ops.get_clauses_wl_from_init_get_clauses_wl_heur_init
+        intro: mset_subset_eq_add_left)
+      by (metis mset_subset_eq_add_left)+
+    subgoal
+      by (auto dest: isasat_input_ops.twl_st_heur_init_vmtf_next_emptyD)
+    subgoal
+      by (auto dest!: isasat_input_ops.twl_st_heur_init_vmtf_fstD)
+    subgoal
+      by (auto simp: get_conflict_wl_is_None_init_def get_conflict_wl_is_None_def
+          split: option.splits)
+    apply assumption+
+    subgoal
+      by (rule isasat_input_ops.twl_st_heur_init_wl)
+    subgoal by fast
+    subgoal by fast
+    subgoal by fast
     subgoal premises p
-      using p(26) \<comment> \<open>only last assumption\<close>
+      using p(29)
       by (auto simp: extract_model_of_state_stat_def extract_model_of_state_def
           isasat_input_ops.twl_st_heur_def get_conflict_wl_is_None_heur_def
           get_conflict_wl_is_None_heur_init_def extract_state_stat_def
           get_conflict_wl_is_None_def split: option.splits)
     done
 qed
-
-thm isasat_input_bounded_nempty.cdcl_twl_stgy_prog_wl_D_heur_break_cdcl_twl_stgy_prog_wl_D
-             [THEN fref_to_Down, unfolded comp_def]
 
 lemma [simp]: \<open>finite (extract_atms_clss CS {})\<close>
   by (auto simp: extract_atms_clss_alt_def)
